src/named/Pf.v
@@ -1,0 +1,401 @@
+Require Import mathcomp.ssreflect.all_ssreflect.
+Set Implicit Arguments.
+Unset Strict Implicit.
+Unset Printing Implicit Defensive.
+Set Bullet Behavior "Strict Subproofs".
+
+Require Import String.
+From Utils Require Import Utils.
+Require Import Named.Exp Named.ARule.
+Import OptionMonad.
+
+(* Proofs of relatedness; todo: separate sort from term pf? *)
+Unset Elimination Schemes.
+Inductive pf : Set :=
+(* variable name; congruence for variables *)
+| pvar : string -> pf
+(* Rule label, list of subterms*)
+(* congruence for constructors *)
+| pcon : string -> list pf -> pf
+(* appealing to a language axiom *)
+| ax : string -> pf
+(* applying a substitution;
+   can't be distributed over axioms
+   unless in the context of a given language
+   
+   TODO: use a named list or regular list?
+   Can I figure out appropriate names given the language?
+   Not in the var case. Should I add a ctx argument to
+   the var case? Seems like it might be a good idea.
+   A relevant is how these terms will be checked.
+   I'll leave this consideration until I get to my proves_wf function.
+
+   TODO: do I want this or no?
+   Might be able to eliminate it, but probably
+   not worth it at the moment.
+ *)
+| sub : pf -> ctx -> list pf -> pf
+| sym : pf -> pf
+| trans : pf -> pf -> pf
+| conv : pf (*term*) -> pf (*sort*) -> pf.
+Set Elimination Schemes.
+
+
+(*Stronger induction principle w/ better subterm knowledge
+ *)
+Fixpoint pf_ind
+         (P : pf -> Prop)
+         (IHV : forall n, P(pvar n))
+         (IHC : forall n l,
+             List.fold_right (fun t => and (P t)) True l ->
+             P (pcon n l))
+         (IHA : forall n, P(ax n))
+         (IHS : forall e' c l,
+             P e' ->
+             List.fold_right (fun p => and (P p)) True l ->
+             P (sub e' c l))
+         (IHSY : forall e', P e' -> P (sym e'))
+         (IHT : forall e1 e2,
+             P e1 -> P e2 -> P (trans e1 e2))
+         (IHCV : forall e1 e2,
+             P e1 -> P e2 -> P (conv e1 e2))
+         (e : pf) { struct e} : P e :=
+  match e with
+  | pvar n => IHV n
+  | pcon n l =>
+    let fix loop l :=
+        match l return List.fold_right (fun t => and (P t)) True l with
+        | [::] => I
+        | e' :: l' => conj (pf_ind IHV IHC IHA IHS IHSY IHT IHCV e') (loop l')
+        end in
+    IHC n l (loop l)
+  | ax n => IHA n
+  | sub e' c l =>
+    let fix loop l :=
+        match l return List.fold_right (fun t => and (P t)) True l with
+        | [::] => I
+        | e' :: l' => conj (pf_ind IHV IHC IHA IHS IHSY IHT IHCV e') (loop l')
+        end in
+    IHS e' c l (pf_ind IHV IHC IHA IHS IHSY IHT IHCV e') (loop l)
+  | sym e' =>
+    IHSY e' (pf_ind IHV IHC IHA IHS IHSY IHT IHCV e')
+  | trans e1 e2 =>
+    IHT e1 e2 (pf_ind IHV IHC IHA IHS IHSY IHT IHCV e1)
+        (pf_ind IHV IHC IHA IHS IHSY IHT IHCV e2)
+  | conv e1 e2 =>
+    IHCV e1 e2 (pf_ind IHV IHC IHA IHS IHSY IHT IHCV e1)
+        (pf_ind IHV IHC IHA IHS IHSY IHT IHCV e2)
+  end.
+
+(* TODO
+Fixpoint exp_rect
+         (P : exp -> Type)
+         (IHV : forall n, P(var n))
+         (IHC : forall n l,
+             List.fold_right (fun t => prod (P t)) unit l ->
+             P (con n l))
+         (e : exp) { struct e} : P e :=
+  match e with
+  | var n => IHV n
+  | con n l =>
+    let fix loop l :=
+        match l return List.fold_right (fun t => prod (P t)) unit l with
+        | [::] => tt
+        | e' :: l' => (exp_rect IHV IHC e', loop l')
+        end in
+    IHC n l (loop l)
+  end.
+
+Definition exp_rec := 
+[eta exp_rect]
+     : forall P : exp -> Set,
+       (forall n, P (var n)) ->
+       (forall n l,
+             List.fold_right (fun t => prod (P t)) unit l ->
+             P (con n l))-> forall e : exp, P e.
+*)
+
+Definition subst_pf : Set := named_list_set pf.
+
+
+(*TODO:move to Utils*)
+Fixpoint get_subseq {A} (args : list string) (l : named_list A) :=
+  match args, l with
+  | [::],_ => do ret [::]
+  | x::args', (x',e)::l' =>
+    if x == x'
+    then do sq <- get_subseq args' l';
+         ret (x,e)::sq
+    else get_subseq args l'
+  | _::_,[::]=> None
+  end.
+             
+Section RuleChecking.
+  Context (l : lang).
+
+  Section InnerLoop.
+    Context (synth_le_term : pf -> ctx -> option (sort*exp*exp)).
+
+    Fixpoint synth_le_args (pl : list pf) (c c' : ctx) {struct pl}
+      : option (list exp * list exp) :=
+      match pl with
+      | [::] => do [::] <- do ret c'; ret ([::],[::])
+      | p::pl' =>
+        do (_,t)::c'' <- do ret c';
+           (t',e1,e2) <- synth_le_term p c;
+           (el1,el2) <- synth_le_args pl' c c'';
+           ! t' == t[/with_names_from c'' el2/];
+           ret (e1::el1, e2::el2)
+     end.
+
+    Fixpoint synth_le_sort (pt : pf) (c : ctx) : option (sort * sort) :=
+      match pt with
+      | pvar x => None
+      | pcon name pl =>
+        do (sort_rule c' args) <- named_list_lookup_err l name;
+           (el1, el2) <- synth_le_args pl c c';
+           al1 <- get_subseq args (with_names_from c' el1);
+           al2 <- get_subseq args (with_names_from c' el2);
+           ret (scon name (map snd al1), scon name (map snd al2))
+      | ax name =>
+        do (sort_le c' e1 e2) <- named_list_lookup_err l name;
+           ! c == c';
+           ret (e1,e2)
+      | sub p c' pl =>
+        do (e1, e2) <- synth_le_sort p c';
+           (el1, el2) <- synth_le_args pl c c';
+           let s1 := with_names_from c' el1;
+           let s2 := with_names_from c' el2;
+           ret (e1[/s1/],e2[/s2/])
+      | sym p =>
+        do (e1,e2) <- synth_le_sort p c;
+           ret (e2,e1)
+      | trans p1 p2 =>
+        do (e1,e2) <- synth_le_sort p1 c;
+           (e2',e3) <- synth_le_sort p2 c;
+           !e2 == e2';
+           ret (e1,e3)
+      | conv pt p => None
+  end.
+
+    Fixpoint synth_le_sort_ex (pt : pf) (c : ctx) : option (sort * sort) :=
+      match pt with
+      | pvar x => None
+      | pcon name pl =>
+        do (sort_rule c' args) <- named_list_lookup_err l name;
+           (el1, el2) <- synth_le_args pl c c';
+           ret (scon name el1, scon name el2)
+      | ax name =>
+        do (sort_le c' e1 e2) <- named_list_lookup_err l name;
+           ! c == c';
+           ret (e1,e2)
+      | sub p c' pl =>
+        do (e1, e2) <- synth_le_sort p c';
+           (el1, el2) <- synth_le_args pl c c';
+           let s1 := with_names_from c' el1;
+           let s2 := with_names_from c' el2;
+           ret (e1[/s1/],e2[/s2/])
+      | sym p =>
+        do (e1,e2) <- synth_le_sort p c;
+           ret (e2,e1)
+      | trans p1 p2 =>
+        do (e1,e2) <- synth_le_sort p1 c;
+           (e2',e3) <- synth_le_sort p2 c;
+           !e2 == e2';
+           ret (e1,e3)
+      | conv pt p => None
+    end.    
+  End InnerLoop.
+
+  (* Defined over proof and implicit terms
+   *)
+  Fixpoint synth_le_term (p : pf) (c : ctx) {struct p} : option (sort*exp*exp) :=
+    match p with
+    | pvar x =>
+      do t <- named_list_lookup_err c x;
+         ret (t,var x, var x)
+    | pcon name pl =>
+      do (term_rule c' args t) <- named_list_lookup_err l name;
+         (el1, el2) <- synth_le_args synth_le_term pl c c';
+         al1 <- get_subseq args (with_names_from c' el1);
+         al2 <- get_subseq args (with_names_from c' el2);
+         ret (t[/with_names_from c' el2/],
+              con name (map snd al1), con name (map snd al2))
+    | ax name =>
+      do (term_le c' e1 e2 t) <- named_list_lookup_err l name;
+         !c == c';
+         ret (t,e1,e2)
+    | sub p' c' pl =>
+      do (t,e1, e2) <- synth_le_term p' c';
+         (el1, el2) <- synth_le_args synth_le_term pl c c';
+         let s1 := with_names_from c' el1;
+         let s2 := with_names_from c' el2;
+         ret (t[/s2/],e1[/s1/],e2[/s2/])
+    | sym p' =>
+      do (t,e1,e2) <- synth_le_term p' c;
+         ret (t,e2,e1)
+    | trans p1 p2 =>
+      do (t,e1,e2) <- synth_le_term p1 c;
+         (t',e2',e3) <- synth_le_term p2 c;
+         ! t == t';
+         ! e2 == e2';
+         ret (t,e1,e3)
+    | conv pt p' =>
+      do (t, e1, e2) <- synth_le_term p' c;
+         (t', t1) <- synth_le_sort synth_le_term pt c;
+         ! t == t';
+         ret (t1,e1,e2)
+  end.
+
+  Fixpoint synth_le_term_ex (p : pf) (c : ctx) {struct p}
+    : option (sort*exp*exp) :=
+    match p with
+    | pvar x =>
+      do t <- named_list_lookup_err c x;
+         ret (t,var x, var x)
+    | pcon name pl =>
+      do (term_rule c' args t) <- named_list_lookup_err l name;
+         (el1, el2) <- synth_le_args synth_le_term_ex pl c c';
+         ret (t[/with_names_from c' el2/],
+              con name el1, con name el2)
+    | ax name =>
+      do (term_le c' e1 e2 t) <- named_list_lookup_err l name;
+         !c == c';
+         ret (t,e1,e2)
+    | sub p' c' pl =>
+      do (t,e1, e2) <- synth_le_term_ex p' c';
+         (el1, el2) <- synth_le_args synth_le_term_ex pl c c';
+         let s1 := with_names_from c' el1;
+         let s2 := with_names_from c' el2;
+         ret (t[/s2/],e1[/s1/],e2[/s2/])
+    | sym p' =>
+      do (t,e1,e2) <- synth_le_term_ex p' c;
+         ret (t,e2,e1)
+    | trans p1 p2 =>
+      do (t,e1,e2) <- synth_le_term_ex p1 c;
+         (t',e2',e3) <- synth_le_term_ex p2 c;
+         ! t == t';
+         ! e2 == e2';
+         ret (t,e1,e3)
+    | conv pt p' =>
+      do (t, e1, e2) <- synth_le_term_ex p' c;
+         (t', t1) <- synth_le_sort_ex synth_le_term_ex pt c;
+         ! t == t';
+         ret (t1,e1,e2)
+  end.
+
+  Definition check_le_term p c t e1 e2 : bool :=
+    synth_le_term p c == Some (t,e1,e2).
+  
+  Definition check_le_sort p c t1 t2 : bool :=
+    synth_le_sort synth_le_term p c == Some (t1,t2).
+
+  Section InnerLoop.
+    Context (synth_wf_term : pf -> ctx -> option (sort*exp)).
+
+    Fixpoint synth_wf_args (pl : list pf) (c c' : ctx) {struct pl}
+      : option (list exp) :=
+      match pl with
+      | [::] => do [::] <- do ret c'; ret ([::])
+      | p::pl' =>
+        do (_,t)::c'' <- do ret c';
+           (t',e) <- synth_wf_term p c;
+           el <- synth_wf_args pl' c c'';
+           ! t' == t[/with_names_from c'' el/];
+           ret (e::el)
+     end.
+  End InnerLoop.
+
+  (* Defined over proof and implicit terms
+   *)
+  Fixpoint synth_wf_term (p : pf) (c : ctx) {struct p} : option (sort*exp) :=
+    match p with
+    | pvar x =>
+      do t <- named_list_lookup_err c x;
+         ret (t,var x)
+    | pcon name pl =>
+      do (term_rule c' args t) <- named_list_lookup_err l name;
+         el <- synth_wf_args synth_wf_term pl c c';
+         al <- get_subseq args (with_names_from c' el);
+         ret (t[/with_names_from c' el/], con name (map snd al))
+    | ax name => None
+    | sub p' c' pl => None
+    | sym p' => None
+    | trans p1 p2 => None
+    | conv pt p' =>
+      do (t, e) <- synth_wf_term p' c;
+         (t', t1) <- synth_le_sort synth_le_term pt c;
+         ! t == t';
+         ret (t1,e)
+  end.
+
+  Definition synth_wf_sort (pt : pf) (c : ctx) : option sort :=
+      match pt with
+      | pvar x => None
+      | pcon name pl =>
+        do (sort_rule c' args) <- named_list_lookup_err l name;
+           el <- synth_wf_args synth_wf_term pl c c';
+           al <- get_subseq args (with_names_from c' el);
+           ret (scon name (map snd al))
+      | ax name => None
+      | sub p c' pl => None
+      | sym p => None
+      | trans p1 p2 => None
+      | conv pt p => None
+    end.
+
+  Definition check_wf_term p c e t : bool :=
+    synth_wf_term p c == Some (t,e).
+  
+  Definition check_wf_sort p c t : bool :=
+    synth_wf_sort p c == Some t.
+
+  Fixpoint check_wf_ctx pl c : bool :=
+    match pl, c with
+    | [::], [::] => true
+    | [::], _::_ => false
+    | _::_,[::] => false
+    | p::pl', (name,t)::c' =>
+      (fresh name c') &&
+      (check_wf_sort p c' t) &&
+      (check_wf_ctx pl' c')
+    end.
+
+  Variant rule_pf : Set :=
+  | sort_rule_pf : list pf -> rule_pf
+  | term_rule_pf : list pf -> pf -> rule_pf
+  | sort_le_pf : list pf -> pf -> pf -> rule_pf
+  | term_le_pf : list pf -> pf -> pf -> pf (*sort*)-> rule_pf.
+      
+  Definition check_wf_rule rp r : bool :=
+    match rp, r with
+    | sort_rule_pf pl, sort_rule c args =>
+      (subseq args (map fst c)) &&
+      (check_wf_ctx pl c)
+    | term_rule_pf pl p, term_rule c args t =>
+      (subseq args (map fst c)) &&
+      (check_wf_ctx pl c) &&
+      (check_wf_sort p c t)
+    | sort_le_pf pl p1 p2, sort_le c t1 t2 =>
+      (check_wf_ctx pl c) &&
+      (check_wf_sort p1 c t1) &&
+      (check_wf_sort p2 c t2)
+    | term_le_pf pl p1 p2 pt, term_le c e1 e2 t =>
+      (check_wf_ctx pl c) &&
+      (check_wf_sort pt c t) &&
+      (check_wf_term p1 c e1 t) &&
+      (check_wf_term p2 c e2 t)
+    | _, _=> false
+    end.
+
+End RuleChecking.
+  
+Fixpoint check_wf_lang rpl l : bool :=
+  match rpl, l with
+  | [::], [::] => true
+  | [::], _::_ => false
+  | _::_,[::] => false
+  | rp::rpl', (name,r)::l' =>
+    (fresh name l') &&
+    (check_wf_rule l' rp r)
+  end.
